src/TrsInv.v
@@ -1,0 +1,81 @@
+Require Import Bool List String Peano_dec.
+Require Import Common FMap ListSupport Syntax Semantics StepM StepT SemFacts.
+Require Import Invariant Serial SerialFacts.
+
+Require Import Omega.
+
+Set Implicit Arguments.
+
+Section TrsInv.
+  Variables (StateI MsgT: Type).
+  Hypothesis (msgT_dec: forall m1 m2: MsgT, {m1 = m2} + {m1 <> m2}).
+  Context `{HasInit System StateI} `{HasMsg MsgT}.
+
+  Variable (impl: System).
+
+  Variables (stepI: Step StateI (RLabel MsgT))
+            (ginv: StateI -> Prop).
+
+  Definition Invariant := @Invariant StateI.
+  Definition InvInit := @InvInit StateI _ impl ginv.
+
+  Definition InvTrs :=
+    forall ist1,
+      ginv ist1 ->
+      forall lbl ist2,
+        trsSteps msgT_dec stepI impl ist1 lbl ist2 ->
+        ginv ist2.
+
+  Definition InvSeq :=
+    forall ist1,
+      ginv ist1 ->
+      forall lbl ist2,
+        seqSteps msgT_dec stepI impl ist1 lbl ist2 ->
+        ginv ist2.
+
+  Hypotheses (Hinvi: InvInit)
+             (Hinvt: InvTrs).
+
+  Lemma inv_trs_seqSteps':
+    forall ist1,
+      ginv ist1 ->
+      forall ihst ist2,
+        seqSteps msgT_dec stepI impl ist1 ihst ist2 ->
+        ginv ist2.
+  Proof.
+    intros.
+    destruct H2; destruct H3 as [trss ?].
+    destruct H3; subst.
+
+    generalize dependent ist2; generalize dependent ist1.
+    induction trss; simpl; intros.
+    - inv H2; assumption.
+    - eapply steps_split in H2; [|reflexivity].
+      destruct H2 as [sti [? ?]].
+      inv H3.
+      eapply Hinvt with (ist1:= sti); eauto.
+      split; eauto.
+  Qed.
+
+  Lemma inv_trs_seqSteps: InvSeq.
+  Proof.
+    unfold InvSeq; intros.
+    eapply inv_trs_seqSteps'; eauto.
+  Qed.
+
+End TrsInv.
+
+Theorem invSeq_serializable_invSteps:
+  forall impl ginv,
+    InvInit impl ginv ->
+    InvSeq msg_dec impl step_m ginv ->
+    SerializableSys impl ->
+    InvSteps impl step_m ginv.
+Proof.
+  unfold InvInit, InvSeq, SerializableSys, InvSteps, Invariant.InvSteps.
+  intros.
+  specialize (H1 _ _ H2).
+  red in H1; destruct H1 as [sll ?].
+  eapply H0; eauto.
+Qed.
+
